fstar/Hacspec.Chacha20.fst
@@ -5,35 +5,33 @@ module Hacspec.Chacha20
 open Hacspec.Lib
 open FStar.Mul
 
-module RSeq = Hacspec.Lib.Seq
-module RNat = Hacspec.Lib.Nat
+type state = lseq (uint32) (usize 16)
 
-type state = RSeq.lseq (uint32) (usize 16)
+type state_bytes = lseq (uint8) (usize 64)
 
-type state_bytes = RSeq.lseq (uint8) (usize 64)
+type iv = lseq (uint8) (usize 12)
 
-type iv = RSeq.lseq (uint8) (usize 12)
-
-type key = RSeq.lseq (uint8) (usize 32)
+type key = lseq (uint8) (usize 32)
 
 let state_to_bytes (x_1870 : state) : state_bytes =
-  let r_1871 = RSeq.new_ 64 () in
+  let r_1871 = seq_new_ 64 in
   let (r_1871) =
-    foldi (usize 0) (RSeq.len (x_1870)) (fun (i_1872, (r_1871)) ->
+    foldi (usize 0) (seq_len (x_1870)) (fun (i_1872, (r_1871)) ->
       let bytes_1873 = uint32_to_be_bytes (array_index (x_1870) (i_1872)) in
       let r_1871 =
-        array_upd r_1871 (i_1872 * usize 4) (array_index (bytes_1873) (usize 3))
+        array_upd r_1871 ((i_1872) * (usize 4)) (
+          array_index (bytes_1873) (usize 3))
       in
       let r_1871 =
-        array_upd r_1871 (i_1872 * usize 4 + usize 1) (
+        array_upd r_1871 (((i_1872) * (usize 4)) + (usize 1)) (
           array_index (bytes_1873) (usize 2))
       in
       let r_1871 =
-        array_upd r_1871 (i_1872 * usize 4 + usize 2) (
+        array_upd r_1871 (((i_1872) * (usize 4)) + (usize 2)) (
           array_index (bytes_1873) (usize 1))
       in
       let r_1871 =
-        array_upd r_1871 (i_1872 * usize 4 + usize 3) (
+        array_upd r_1871 (((i_1872) * (usize 4)) + (usize 3)) (
           array_index (bytes_1873) (usize 0))
       in
       (r_1871))
@@ -51,15 +49,17 @@ let line
   let state_1879 = m_1878 in
   let state_1879 =
     array_upd state_1879 (a_1874) (
-      array_index (state_1879) (a_1874) +. array_index (state_1879) (b_1875))
+      (array_index (state_1879) (a_1874)) +. (
+        array_index (state_1879) (b_1875)))
   in
   let state_1879 =
     array_upd state_1879 (d_1876) (
-      array_index (state_1879) (d_1876) ^. array_index (state_1879) (a_1874))
+      (array_index (state_1879) (d_1876)) ^. (
+        array_index (state_1879) (a_1874)))
   in
   let state_1879 =
     array_upd state_1879 (d_1876) (
-      U32.rotate_left (array_index (state_1879) (d_1876)) (s_1877))
+      uint32_rotate_left (array_index (state_1879) (d_1876)) (s_1877))
   in
   state_1879
 
@@ -108,34 +108,34 @@ let double_round (state_1888 : state) : state =
     state_1895)
 
 let block_init (key_1896 : key) (ctr_1897 : uint32) (iv_1898 : iv) : state =
-  RSeq.from_list [
+  seq_from_list [
     secret (pub_u32 0x61707865);
     secret (pub_u32 0x3320646e);
     secret (pub_u32 0x79622d32);
     secret (pub_u32 0x6b206574);
     uint32_from_le_bytes (
-      RSeq.from_slice_range 4 (key_1896) ((usize 0, usize 4)));
+      seq_from_slice_range 4 (key_1896) ((usize 0, usize 4)));
     uint32_from_le_bytes (
-      RSeq.from_slice_range 4 (key_1896) ((usize 4, usize 8)));
+      seq_from_slice_range 4 (key_1896) ((usize 4, usize 8)));
     uint32_from_le_bytes (
-      RSeq.from_slice_range 4 (key_1896) ((usize 8, usize 12)));
+      seq_from_slice_range 4 (key_1896) ((usize 8, usize 12)));
     uint32_from_le_bytes (
-      RSeq.from_slice_range 4 (key_1896) ((usize 12, usize 16)));
+      seq_from_slice_range 4 (key_1896) ((usize 12, usize 16)));
     uint32_from_le_bytes (
-      RSeq.from_slice_range 4 (key_1896) ((usize 16, usize 20)));
+      seq_from_slice_range 4 (key_1896) ((usize 16, usize 20)));
     uint32_from_le_bytes (
-      RSeq.from_slice_range 4 (key_1896) ((usize 20, usize 24)));
+      seq_from_slice_range 4 (key_1896) ((usize 20, usize 24)));
     uint32_from_le_bytes (
-      RSeq.from_slice_range 4 (key_1896) ((usize 24, usize 28)));
+      seq_from_slice_range 4 (key_1896) ((usize 24, usize 28)));
     uint32_from_le_bytes (
-      RSeq.from_slice_range 4 (key_1896) ((usize 28, usize 32)));
+      seq_from_slice_range 4 (key_1896) ((usize 28, usize 32)));
     ctr_1897;
     uint32_from_le_bytes (
-      RSeq.from_slice_range 4 (iv_1898) ((usize 0, usize 4)));
+      seq_from_slice_range 4 (iv_1898) ((usize 0, usize 4)));
     uint32_from_le_bytes (
-      RSeq.from_slice_range 4 (iv_1898) ((usize 4, usize 8)));
+      seq_from_slice_range 4 (iv_1898) ((usize 4, usize 8)));
     uint32_from_le_bytes (
-      RSeq.from_slice_range 4 (iv_1898) ((usize 8, usize 12)))
+      seq_from_slice_range 4 (iv_1898) ((usize 8, usize 12)))
   ]
 
 let block_inner (key_1899 : key) (ctr_1900 : uint32) (iv_1901 : iv) : state =
@@ -151,7 +151,8 @@ let block_inner (key_1899 : key) (ctr_1900 : uint32) (iv_1901 : iv) : state =
     foldi (usize 0) (usize 16) (fun (i_1905, (state_1903)) ->
       let state_1903 =
         array_upd state_1903 (i_1905) (
-          array_index (state_1903) (i_1905) +. array_index (st_1902) (i_1905))
+          (array_index (state_1903) (i_1905)) +. (
+            array_index (st_1902) (i_1905)))
       in
       (state_1903))
     (state_1903)
@@ -164,28 +165,28 @@ let block (key_1906 : key) (ctr_1907 : uint32) (iv_1908 : iv) : state_bytes =
 
 let chacha (key_1910 : key) (iv_1911 : iv) (m_1912 : byte_seq) : byte_seq =
   let ctr_1913 = secret (pub_u32 0x1) in
-  let blocks_out_1914 = RSeq.new_ (RSeq.len (m_1912)) in
-  let (ctr_1913, blocks_out_1914) =
-    foldi (usize 0) (RSeq.num_chunks (m_1912) (usize 64)) (fun (
+  let blocks_out_1914 = seq_new_ (seq_len (m_1912)) in
+  let (blocks_out_1914, ctr_1913) =
+    foldi (usize 0) (seq_num_chunks (m_1912) (usize 64)) (fun (
         i_1915,
-        (ctr_1913, blocks_out_1914)
+        (blocks_out_1914, ctr_1913)
       ) ->
       let (block_len_1916, msg_block_1917) =
-        RSeq.get_chunk (m_1912) (usize 64) (i_1915)
+        seq_get_chunk (m_1912) (usize 64) (i_1915)
       in
       let key_block_1918 = block (key_1910) (ctr_1913) (iv_1911) in
-      let msg_block_padded_1919 = RSeq.new_ 64 () in
+      let msg_block_padded_1919 = seq_new_ 64 in
       let msg_block_padded_1920 =
-        RSeq.update_start (msg_block_padded_1919) (msg_block_1917)
+        seq_update_start (msg_block_padded_1919) (msg_block_1917)
       in
       let blocks_out_1914 =
-        RSeq.set_chunk #uint8 (blocks_out_1914) (usize 64) (i_1915) (
-          RSeq.slice_range (msg_block_padded_1920 ^. key_block_1918) (
+        seq_set_chunk #uint8 (blocks_out_1914) (usize 64) (i_1915) (
+          seq_slice_range ((msg_block_padded_1920) `seq_xor` (key_block_1918)) (
             (usize 0, block_len_1916)))
       in
-      let ctr_1913 = ctr_1913 +. secret (pub_u32 0x1) in
-      (ctr_1913, blocks_out_1914))
-    (ctr_1913, blocks_out_1914)
+      let ctr_1913 = (ctr_1913) +. (secret (pub_u32 0x1)) in
+      (blocks_out_1914, ctr_1913))
+    (blocks_out_1914, ctr_1913)
   in
   blocks_out_1914
 
