fstar/Hacspec.NtruDemo.fst
@@ -5,32 +5,29 @@ module Hacspec.NtruDemo
 open Hacspec.Lib
 open FStar.Mul
 
-module RSeq = Hacspec.Lib.Seq
-module RNat = Hacspec.Lib.Nat
-
-let build_irreducible (p_1842 : uint_size) : RSeq.seq pub_int128 =
-  let irr_1843 = RSeq.new_ #pub_int128 (p_1842 + usize 1) in
-  let irr_1843 = array_upd irr_1843 (usize 0) (- pub_i128 0x1) in
-  let irr_1843 = array_upd irr_1843 (usize 1) (- pub_i128 0x1) in
+let build_irreducible (p_1842 : uint_size) : seq pub_int128 =
+  let irr_1843 = seq_new_ #pub_int128 ((p_1842) + (usize 1)) in
+  let irr_1843 = array_upd irr_1843 (usize 0) (- (pub_i128 0x1)) in
+  let irr_1843 = array_upd irr_1843 (usize 1) (- (pub_i128 0x1)) in
   let irr_1843 = array_upd irr_1843 (p_1842) (pub_i128 0x1) in
   irr_1843
 
 let round_to_3
-  (poly_1844 : RSeq.seq pub_int128)
+  (poly_1844 : seq pub_int128)
   (q_1845 : pub_int128)
-  : RSeq.seq pub_int128 =
-  let result_1846 = RSeq.clone #pub_int128 (poly_1844) in
-  let q_12_1847 = q_1845 -. pub_i128 0x1 /. pub_i128 0x2 in
+  : seq pub_int128 =
+  let result_1846 = seq_clone #pub_int128 (poly_1844) in
+  let q_12_1847 = ((q_1845) -. (pub_i128 0x1)) /. (pub_i128 0x2) in
   let (result_1846) =
-    foldi (usize 0) (RSeq.len #pub_int128 (poly_1844)) (fun (
+    foldi (usize 0) (seq_len #pub_int128 (poly_1844)) (fun (
         i_1848,
         (result_1846)
       ) ->
       let (result_1846) =
-        if array_index (poly_1844) (i_1848) >. q_12_1847 then begin
+        if (array_index (poly_1844) (i_1848)) >. (q_12_1847) then begin
           let result_1846 =
             array_upd result_1846 (i_1848) (
-              array_index (poly_1844) (i_1848) -. q_1845)
+              (array_index (poly_1844) (i_1848)) -. (q_1845))
           in
           (result_1846)
         end else begin (result_1846)
@@ -40,23 +37,23 @@ let round_to_3
     (result_1846)
   in
   let (result_1846) =
-    foldi (usize 0) (RSeq.len #pub_int128 (result_1846)) (fun (
+    foldi (usize 0) (seq_len #pub_int128 (result_1846)) (fun (
         i_1849,
         (result_1846)
       ) ->
       let (result_1846) =
-        if array_index (result_1846) (
-          i_1849) %. pub_i128 0x3 != pub_i128 0x0 then begin
+        if ((array_index (result_1846) (i_1849)) %. (pub_i128 0x3)) != (
+          pub_i128 0x0) then begin
           let result_1846 =
             array_upd result_1846 (i_1849) (
-              array_index (result_1846) (i_1849) -. pub_i128 0x1)
+              (array_index (result_1846) (i_1849)) -. (pub_i128 0x1))
           in
           let (result_1846) =
-            if array_index (result_1846) (
-              i_1849) %. pub_i128 0x3 != pub_i128 0x0 then begin
+            if ((array_index (result_1846) (i_1849)) %. (pub_i128 0x3)) != (
+              pub_i128 0x0) then begin
               let result_1846 =
                 array_upd result_1846 (i_1849) (
-                  array_index (result_1846) (i_1849) +. pub_i128 0x2)
+                  (array_index (result_1846) (i_1849)) +. (pub_i128 0x2))
               in
               (result_1846)
             end else begin (result_1846)
@@ -72,18 +69,18 @@ let round_to_3
   result_1846
 
 let encrypt
-  (r_1850 : RSeq.seq pub_int128)
-  (h_1851 : RSeq.seq pub_int128)
+  (r_1850 : seq pub_int128)
+  (h_1851 : seq pub_int128)
   (q_1852 : pub_int128)
-  (irreducible_1853 : RSeq.seq pub_int128)
-  : RSeq.seq pub_int128 =
+  (irreducible_1853 : seq pub_int128)
+  : seq pub_int128 =
   let pre_1854 = mul_poly_irr (r_1850) (h_1851) (irreducible_1853) (q_1852) in
   round_to_3 (pre_1854) (q_1852)
 
 let ntru_prime_653_encrypt
-  (r_1855 : RSeq.seq pub_int128)
-  (h_1856 : RSeq.seq pub_int128)
-  : RSeq.seq pub_int128 =
+  (r_1855 : seq pub_int128)
+  (h_1856 : seq pub_int128)
+  : seq pub_int128 =
   let p_1857 = usize 653 in
   let q_1858 = pub_i128 0x120d in
   let w_1859 = usize 288 in
@@ -91,10 +88,10 @@ let ntru_prime_653_encrypt
   encrypt (r_1855) (h_1856) (q_1858) (irreducible_1860)
 
 let ntru_prime_653_decrypt
-  (c_1861 : RSeq.seq pub_int128)
-  (key_f_1862 : RSeq.seq pub_int128)
-  (key_v_1863 : RSeq.seq pub_int128)
-  : (RSeq.seq pub_int128 & bool) =
+  (c_1861 : seq pub_int128)
+  (key_f_1862 : seq pub_int128)
+  (key_v_1863 : seq pub_int128)
+  : (seq pub_int128 & bool) =
   let p_1864 = usize 653 in
   let q_1865 = pub_i128 0x120d in
   let w_1866 = usize 288 in
@@ -109,17 +106,17 @@ let ntru_prime_653_decrypt
   in
   let (f_3_c_1870, ok_decrypt_1871) = f_3_c_and_decryption_ok_1869 in
   let f_3_c_1872 = f_3_c_1870 in
-  let q_12_1873 = q_1865 -. pub_i128 0x1 /. pub_i128 0x2 in
+  let q_12_1873 = ((q_1865) -. (pub_i128 0x1)) /. (pub_i128 0x2) in
   let (f_3_c_1872) =
-    foldi (usize 0) (RSeq.len #pub_int128 (f_3_c_1872)) (fun (
+    foldi (usize 0) (seq_len #pub_int128 (f_3_c_1872)) (fun (
         i_1874,
         (f_3_c_1872)
       ) ->
       let (f_3_c_1872) =
-        if array_index (f_3_c_1872) (i_1874) >. q_12_1873 then begin
+        if (array_index (f_3_c_1872) (i_1874)) >. (q_12_1873) then begin
           let f_3_c_1872 =
             array_upd f_3_c_1872 (i_1874) (
-              array_index (f_3_c_1872) (i_1874) -. q_1865)
+              (array_index (f_3_c_1872) (i_1874)) -. (q_1865))
           in
           (f_3_c_1872)
         end else begin (f_3_c_1872)
@@ -128,12 +125,12 @@ let ntru_prime_653_decrypt
       (f_3_c_1872))
     (f_3_c_1872)
   in
-  let e_1875 = RSeq.new_ #pub_int128 (RSeq.len #pub_int128 (f_3_c_1872)) in
+  let e_1875 = seq_new_ #pub_int128 (seq_len #pub_int128 (f_3_c_1872)) in
   let (e_1875) =
-    foldi (usize 0) (RSeq.len #pub_int128 (e_1875)) (fun (i_1876, (e_1875)) ->
+    foldi (usize 0) (seq_len #pub_int128 (e_1875)) (fun (i_1876, (e_1875)) ->
       let e_1875 =
         array_upd e_1875 (i_1876) (
-          array_index (f_3_c_1872) (i_1876) %. pub_i128 0x3)
+          (array_index (f_3_c_1872) (i_1876)) %. (pub_i128 0x3))
       in
       (e_1875))
     (e_1875)
@@ -143,10 +140,10 @@ let ntru_prime_653_decrypt
     mul_poly_irr (e_1875) (key_v_1863) (irreducible_1867) (pub_i128 0x3)
   in
   let (r_1877) =
-    foldi (usize 0) (RSeq.len #pub_int128 (r_1877)) (fun (i_1878, (r_1877)) ->
+    foldi (usize 0) (seq_len #pub_int128 (r_1877)) (fun (i_1878, (r_1877)) ->
       let (r_1877) =
-        if array_index (r_1877) (i_1878) == pub_i128 0x2 then begin
-          let r_1877 = array_upd r_1877 (i_1878) (- pub_i128 0x1) in
+        if (array_index (r_1877) (i_1878)) == (pub_i128 0x2) then begin
+          let r_1877 = array_upd r_1877 (i_1878) (- (pub_i128 0x1)) in
           (r_1877)
         end else begin (r_1877)
         end
