fstar/Hacspec.Poly1305.fst
@@ -5,50 +5,47 @@ module Hacspec.Poly1305
 open Hacspec.Lib
 open FStar.Mul
 
-module RSeq = Hacspec.Lib.Seq
-module RNat = Hacspec.Lib.Nat
-
-type key_poly = RSeq.lseq (uint8) (usize 32)
+type key_poly = lseq (uint8) (usize 32)
 
 let blocksize : uint_size =
   usize 16
 
-type block = RSeq.lseq (uint8) (blocksize)
+type block = lseq (uint8) (blocksize)
 
-type tag = RSeq.lseq (pub_uint8) (blocksize)
+type tag = lseq (pub_uint8) (blocksize)
 
-type field_canvas = RSeq.lseq (pub_uint8) (usize 272)
+type field_canvas = lseq (pub_uint8) (usize 272)
 
 type field_element = nat_mod 0x03fffffffffffffffffffffffffffffffb
 
 let encode_r (r_1864 : block) : field_element =
-  let r_128_1865 = RSeq.from_slice 16 (r_1864) (usize 0) (blocksize) in
+  let r_128_1865 = seq_from_slice 16 (r_1864) (usize 0) (blocksize) in
   let r_uint_1866 = uint128_from_le_bytes (r_128_1865) in
   let r_uint_1867 =
-    r_uint_1866 &. secret (pub_u128 0xffffffc0ffffffc0ffffffc0fffffff)
+    (r_uint_1866) &. (secret (pub_u128 0xffffffc0ffffffc0ffffffc0fffffff))
   in
-  RNat.from_secret_literal (r_uint_1867)
+  nat_from_secret_literal (r_uint_1867)
 
 let encode (block_1868 : byte_seq) : field_element =
-  let block_len_1869 = RSeq.len (block_1868) in
+  let block_len_1869 = seq_len (block_1868) in
   let block_as_u128_1870 =
-    RSeq.from_slice 16 (block_1868) (usize 0) (min (usize 16) (block_len_1869))
+    seq_from_slice 16 (block_1868) (usize 0) (min (usize 16) (block_len_1869))
   in
   let w_elem_1871 =
-    RNat.from_secret_literal (uint128_from_le_bytes (block_as_u128_1870))
+    nat_from_secret_literal (uint128_from_le_bytes (block_as_u128_1870))
   in
-  let l_elem_1872 = RNat.pow2 (usize 8 * block_len_1869) in
-  w_elem_1871 + l_elem_1872
+  let l_elem_1872 = nat_pow2 ((usize 8) * (block_len_1869)) in
+  (w_elem_1871) + (l_elem_1872)
 
 let poly_inner (m_1873 : byte_seq) (r_1874 : field_element) : field_element =
-  let acc_1875 = RNat.from_literal (pub_u128 0x0) in
+  let acc_1875 = nat_from_literal (pub_u128 0x0) in
   let (acc_1875) =
-    foldi (usize 0) (RSeq.num_chunks (m_1873) (blocksize)) (fun (
+    foldi (usize 0) (seq_num_chunks (m_1873) (blocksize)) (fun (
         i_1876,
         (acc_1875)
       ) ->
-      let (_, block_1877) = RSeq.get_chunk (m_1873) (blocksize) (i_1876) in
-      let acc_1875 = acc_1875 + encode (block_1877) * r_1874 in
+      let (_, block_1877) = seq_get_chunk (m_1873) (blocksize) (i_1876) in
+      let acc_1875 = ((acc_1875) + (encode (block_1877))) * (r_1874) in
       (acc_1875))
     (acc_1875)
   in
@@ -56,20 +53,20 @@ let poly_inner (m_1873 : byte_seq) (r_1874 : field_element) : field_element =
 
 let poly (m_1878 : byte_seq) (key_1879 : key_poly) : tag =
   let s_elem_1880 =
-    RNat.from_secret_literal (
+    nat_from_secret_literal (
       uint128_from_le_bytes (
-        RSeq.from_slice 16 (key_1879) (blocksize) (blocksize)))
+        seq_from_slice 16 (key_1879) (blocksize) (blocksize)))
   in
   let r_elem_1881 =
-    encode_r (RSeq.from_slice_range blocksize (key_1879) ((usize 0, blocksize)))
+    encode_r (seq_from_slice_range blocksize (key_1879) ((usize 0, blocksize)))
   in
   let a_1882 = poly_inner (m_1878) (r_elem_1881) in
-  let n_1883 = a_1882 + s_elem_1880 in
-  let n_v_1884 = RNat.to_public_byte_seq_le (n_1883) in
-  let tag_1885 = RSeq.new_ blocksize () in
+  let n_1883 = (a_1882) + (s_elem_1880) in
+  let n_v_1884 = nat_to_public_byte_seq_le (n_1883) in
+  let tag_1885 = seq_new_ blocksize in
   let (tag_1885) =
     foldi (usize 0) (
-        min (RSeq.len (tag_1885)) (RSeq.len #pub_uint8 (n_v_1884))) (fun (
+        min (seq_len (tag_1885)) (seq_len #pub_uint8 (n_v_1884))) (fun (
         i_1886,
         (tag_1885)
       ) ->
